redone gain

dp/6_4.dfy
@@ -29,17 +29,10 @@
 
 predicate greedy_a1(S: string, i: nat, j: nat)
 decreases |S| - i, |S| - j 
-requires 0 <= i <= j <= |S|
+requires 0 <= i < j <= |S|
 {
-    if i <= j < |S|-1 then
-        if dict(S[i..j+1]) then
-        //true else false
-            if greedy_a1(S, j+1, j+1) then
-                true else false
-        else if greedy_a1(S, i, j+1) then
-            true else false
-    //else dict(S[i..j]) 
-    else if j < |S| then dict(S[i..j])  else false
+    if j == |S| then dict(S[i..j]) else
+    greedy_a1(S,i,j+1) 
 }
 
 // Limited dictionary function.
@@ -52,6 +45,17 @@ method Main()
 {
     assert dict("a");
     assert dict("s") == false;
-    assert greedy_a1("a", 0, 0) == true;
-    assert greedy_a1("asx", 0, 0) == true;
+    var a1 := "a";
+    var a1' := a1[0..1];
+    assert |a1[0..1]| == 1;
+    assert a1[0..1] == "a";
+    assert dict(a1);
+    //var a2 := "aa";
+    assert greedy_a1("a", 0, 1) == true;
+    assert "as"[0..2] == "as";
+    assert dict("as"[0..2]);
+    assert greedy_a1("as", 0, 1) == true;
+    assert "asa"[0..3] == "asa";
+    assert greedy_a1("asa", 0, 1) == true;
+    //assert greedy_a1("asx", 0, 0) == false;
 }
